More systematic construction for the partitioning of final states.

theories/modules/EventPartitioning.ec
@@ -10,15 +10,17 @@ module type T = {
   proc f(_: input): output
 }.
 
-abstract theory Partitioning.
+abstract theory ListPartitioning.
   type partition.
 
   section.
   declare module M : T.
 
-  lemma probability_partitioning
-          &m i (E : input -> (glob M) -> output -> bool)
-          (phi : input -> (glob M) -> output -> partition) P:
+  lemma list_partitioning
+          (i : input)
+          (E : input -> (glob M) -> output -> bool)
+          (phi : input -> (glob M) -> output -> partition)
+          (P : partition list) &m:
     uniq P =>
     Pr[M.f(i) @ &m: E i (glob M) res]
     = big predT (fun a =>
@@ -37,56 +39,139 @@ abstract theory Partitioning.
   by rewrite Pr[mu_false] //= big_cons {1}/predT /=; congr; exact/ih.
   qed.
   end section.
-end Partitioning.
+end ListPartitioning.
 
-theory TotalResultPartitioning.
+abstract theory FSetPartitioning.
+  require import FSet.
+
+  type partition.
+
   section.
   declare module M : T.
 
-  local clone import Partitioning with type partition <- output.
+  local clone import ListPartitioning with
+    type partition <- partition.
 
-  lemma Pr_support_split &m i X (E : input -> (glob M) -> output -> bool):
+  lemma fset_partitioning
+          (i : input)
+          (E : input -> (glob M) -> output -> bool)
+          (phi : input -> (glob M) -> output -> partition)
+          (P : partition fset) &m:
+    Pr[M.f(i) @ &m: E i (glob M) res]
+    = big predT (fun a =>
+                   Pr[M.f(i) @ &m: E i (glob M) res /\ phi i (glob M) res = a]) (elems P)
+      + Pr[M.f(i) @ &m: E i (glob M) res /\ !mem P (phi i (glob M) res)].
+  proof.
+  by rewrite memE; exact/(@list_partitioning M i E phi (elems P) &m _)/uniq_elems.
+  qed.
+  end section.
+end FSetPartitioning.
+
+abstract theory FPredPartitioning.
+  require import Finite.
+
+  type partition.
+
+  section.
+  declare module M : T.
+
+  local clone import ListPartitioning with
+    type partition <- partition.
+
+  lemma fpred_partitioning
+          (i : input)
+          (E : input -> (glob M) -> output -> bool)
+          (phi : input -> (glob M) -> output -> partition)
+          (P : partition -> bool) &m:
+    is_finite P =>
+    Pr[M.f(i) @ &m: E i (glob M) res]
+    = big predT (fun a =>
+                   Pr[M.f(i) @ &m: E i (glob M) res /\ phi i (glob M) res = a]) (to_seq P)
+      + Pr[M.f(i) @ &m: E i (glob M) res /\ !P (phi i (glob M) res)].
+  proof.
+  move=> ^/mem_to_seq <- /uniq_to_seq.
+  exact/(@list_partitioning M i E phi (to_seq P) &m).
+  qed.
+  end section.
+end FPredPartitioning.
+
+theory ResultPartitioning.
+  section.
+  declare module M : T.
+
+  local clone import ListPartitioning with
+    type partition <- output.
+
+  lemma result_partitioning
+          (i : input)
+          (E : input -> (glob M) -> output -> bool)
+          (X : input -> output list)
+          &m:
+    Pr[M.f(i) @ &m: E i (glob M) res]
+    = big predT (fun a=> Pr[M.f(i) @ &m: E i (glob M) res /\ res = a]) (undup (X i))
+      + Pr[M.f(i) @ &m: E i (glob M) res /\ !mem (X i) res].
+  proof.
+  rewrite -mem_undup.
+  exact/(@list_partitioning M i E (fun _ _ x=> x) (undup (X i)) &m)/undup_uniq.
+  qed.
+  end section.
+end ResultPartitioning.
+
+theory TotalResultPartitioning.
+  (*---*) import ResultPartitioning.
+
+  section.
+  declare module M : T.
+
+  lemma total_result_partitioning
+          (i : input)
+          (E : input -> (glob M) -> output -> bool)
+          (X : input -> output list)
+          &m:
     (forall i, hoare [M.f: arg = i ==> mem (X i) res]) =>
     Pr[M.f(i) @ &m: E i (glob M) res]
     = big predT (fun a => Pr[M.f(i) @ &m: E i (glob M) res /\ res = a]) (undup (X i)).
   proof.
   move=> support_M.
-  rewrite (@probability_partitioning M &m i E (fun _ _ x => x) (undup (X i))) 1:undup_uniq.
-  have ->: Pr[M.f(i) @ &m: E i (glob M) res /\ !mem (undup (X i)) res]
+  rewrite (@result_partitioning M i E X &m).
+  have ->: Pr[M.f(i) @ &m: E i (glob M) res /\ !mem (X i) res]
            = Pr[M.f(i) @ &m: false].
     rewrite Pr[mu_false]; byphoare (_: arg = i ==> _)=> //=.
-    by hoare; conseq (support_M i)=> /> &hr r gm; rewrite mem_undup=> />.
+    by hoare; conseq (support_M i)=> />.
   by rewrite Pr[mu_false].
   qed.
   end section.
 end TotalResultPartitioning.
 
-theory TotalSubuniformPartitioning.
+theory TotalSubuniformResultOnly.
+  import TotalResultPartitioning.
+
   section.
   declare module M : T.
 
-  axiom M_subuniform a b X &m i:
+  axiom M_suf a b i X &m:
        mem (X i) a
     => mem (X i) b
     => Pr[M.f(i) @ &m: res = a] = Pr[M.f(i) @ &m: res = b].
 
-  lemma Pr_subuniform_split &m i X a:
+  lemma subuniform_result i X a &m:
        (forall i, hoare [M.f: arg = i ==> mem (X i) res])
     => mem (X i) a
     => Pr[M.f(i) @ &m: true] = (size (undup (X i)))%r * Pr[M.f(i) @ &m: res = a].
   proof.
   move=> support_M a_in_X.
   rewrite
-    (@TotalResultPartitioning.Pr_support_split M &m i X (fun _ _=> predT)) //
+    (@total_result_partitioning M i (fun _ _=> predT) X &m) //
     big_seq (@eq_bigr _ _ (fun b=> Pr[M.f(i) @ &m: res = a])).
-  + by move=> b /=; rewrite mem_undup=> b_in_X; apply/(@M_subuniform b a X &m i).
+  + by move=> b /=; rewrite mem_undup=> b_in_X; exact/(@M_suf b a i X &m).
   rewrite -big_seq big_const count_predT -AddMonoid.iteropE -intmulpE 1:size_ge0.
   by rewrite intmulr mulrC.
   qed.
   end section.
-end TotalSubuniformPartitioning.
+end TotalSubuniformResultOnly.
 
-theory ScaledUniformByResult.
+theory SubuniformReference.
+  import TotalSubuniformResultOnly.
   (*---*) import MUniform DScalar.
 
   (* "fun i=> Pr[M.f(i) @ &m: true]" is not well-defined because of &m *)
@@ -95,18 +180,26 @@ theory ScaledUniformByResult.
   lemma gt0_k i: 0%r < k i  by move: (k_in_unit i).
   lemma le1_k i: k i <= 1%r by move: (k_in_unit i).
 
-  (* The first few Sections are more general than this: generalize them and push them out? *)
+  module Ref = {
+    proc f(i : input, xs : output list): output = {
+      var r;
+
+      r <$ (k i) \cdot (duniform xs);
+      return r;
+    }
+  }.
+
   section.
   declare module M : T.
 
-  axiom M_subuniform a b X &m i:
+  axiom M_suf a b i X &m:
        mem (X i) a
     => mem (X i) b
     => Pr[M.f(i) @ &m: res = a] = Pr[M.f(i) @ &m: res = b].
 
   axiom weight_M: phoare [M.f: true ==> true] =(k arg).
 
-  lemma Pr_a_notin_X &m i X a:
+  lemma pr_res_notin_X a i X &m:
        (forall i, hoare [M.f: arg = i ==> mem (X i) res])
     => !mem (X i) a
     => Pr[M.f(i) @ &m: res = a] = 0%r.
@@ -116,45 +209,37 @@ theory ScaledUniformByResult.
   by apply/(@contra (r = a) (!mem (X arg{hr}) r))=> ->.
   qed.
 
-  lemma Pr_uniform &m i X a:
+  lemma is_subuniform i X a &m:
        (forall i, hoare [M.f: arg = i ==> mem (X i) res])
     => mem (X i) a
     => Pr[M.f(i) @ &m: res = a] = (k i)/(size (undup (X i)))%r.
   proof.
   move=> support_M a_in_X; have <-: Pr[M.f(i) @ &m: true] = (k i).
   + by byphoare (_: arg = i ==> true)=> //=; conseq weight_M.
-  rewrite (@TotalSubuniformPartitioning.Pr_subuniform_split M M_subuniform &m i X a support_M a_in_X) mulrAC divff //.
+  rewrite (@subuniform_result M M_suf i X a &m support_M a_in_X) mulrAC divff //.
   rewrite eq_fromint size_eq0 undup_nilp -implybF=> h.
   by move: a_in_X; rewrite h.
   qed.
 
-  module Reference = {
-    proc f(i: input, xs : input -> output list): output = {
-      var r;
-
-      r <$ (k i) \cdot (duniform (xs i));
-      return r;
-    }
-  }.
-
-  lemma M_uniform &m X:
+  lemma eq_M_Ref &m X:
        (forall i, hoare [M.f: arg = i ==> mem (X i) res])
     => (forall i, X i <> [])
-    => equiv [M.f ~ Reference.f: arg{1} = i{2} /\ xs{2} = X ==> ={res}].
+    => equiv [M.f ~ Ref.f: (i,xs){2} = (arg,X arg){1} ==> ={res}].
   proof.
   move=> support_M Xi_neq0.
-  bypr (res{1}) (res{2})=> //= &1 &2 a [] i_def xs.
+  bypr (res{1}) (res{2})=> //= &1 &2 a [] i_def xs_def.
   rewrite !(@eq_sym a); case: (mem (X arg{1}) a); last first.
-  + move=> ^a_notin_X /(@Pr_a_notin_X &1 arg{1} X a support_M) ->.
-    byphoare (_: arg = (i,xs){2} ==> _)=> //=; hoare; proc; auto=> /> r.
+  + move=> ^a_notin_X /(@pr_res_notin_X a arg{1} X &1 support_M) ->.
+    byphoare (_: (i,xs) = (arg,X arg){1} ==> _)=> //=.
+    hoare; proc; auto=> /> r.
     rewrite -/(support _ _) support_dscalar_gt0 1:gt0_k.
-    + by rewrite duniform_ll 1:xs 1:Xi_neq0 // le1_k.
-    by case: (r = a)=> [->|]; first by rewrite xs -i_def duniform_fu.
-  move=> a_in_X. rewrite (@Pr_uniform &1 arg{1} X a support_M a_in_X).
-  byphoare (_: arg = (i,xs){2} ==> _)=> //=; proc; rnd (pred1 a); auto=> />.
-  rewrite -i_def xs dscalar1E 1:ltrW 1:gt0_k.
-  + by rewrite duniform_ll 1:Xi_neq0 //= le1_k.
-  by rewrite duniform1E a_in_X.
+    + by rewrite duniform_ll 1:Xi_neq0 // le1_k.
+    by case: (r = a)=> [->|]; first by rewrite duniform_fu.
+  move=> a_in_X. rewrite (@is_subuniform arg{1} X a &1 support_M a_in_X).
+  byphoare (_: (i,xs) = (i,xs){2} ==> _)=> //=; proc; rnd (pred1 a); auto=> />.
+  rewrite dscalar1E 1:ltrW 1:gt0_k.
+  + by rewrite duniform_ll 1:xs_def 1:Xi_neq0 //= le1_k.
+  by rewrite duniform1E i_def xs_def a_in_X.
   qed.
   end section.
-end ScaledUniformByResult.
+end SubuniformReference.
